\documentclass{article}
\parindent 0pt
\begin{document}
${\mathcal A}^{(1)}_{z} =
2\sqrt{\pi/3}Y_{1,0}$\\
${\mathcal A}^{(1)}_{y} =
i\sqrt{2\pi/3}Y_{1,1}
 +i\sqrt{2\pi/3}Y_{1,-1}$\\
${\mathcal A}^{(1)}_{x} =
 -\sqrt{2\pi/3}Y_{1,1}
 +\sqrt{2\pi/3}Y_{1,-1}$\\
${\mathcal A}^{(2)}_{zz} =
(4/3)\sqrt{\pi/5}Y_{2,0}$\\
${\mathcal A}^{(2)}_{yz} =
i\sqrt{2\pi/15}Y_{2,1}
 +i\sqrt{2\pi/15}Y_{2,-1}$\\
${\mathcal A}^{(2)}_{yy} =
 -\sqrt{2\pi/15}Y_{2,2}
 -(2/3)\sqrt{\pi/5}Y_{2,0}
 -\sqrt{2\pi/15}Y_{2,-2}$\\
${\mathcal A}^{(2)}_{xz} =
 -\sqrt{2\pi/15}Y_{2,1}
 +\sqrt{2\pi/15}Y_{2,-1}$\\
${\mathcal A}^{(2)}_{xy} =
 -i\sqrt{2\pi/15}Y_{2,2}
 +i\sqrt{2\pi/15}Y_{2,-2}$\\
${\mathcal A}^{(2)}_{xx} =
\sqrt{2\pi/15}Y_{2,2}
 -(2/3)\sqrt{\pi/5}Y_{2,0}
 +\sqrt{2\pi/15}Y_{2,-2}$\\
${\mathcal A}^{(3)}_{zzz} =
(4/5)\sqrt{\pi/7}Y_{3,0}$\\
${\mathcal A}^{(3)}_{yzz} =
(4i/5)\sqrt{\pi/21}Y_{3,1}
 +(4i/5)\sqrt{\pi/21}Y_{3,-1}$\\
${\mathcal A}^{(3)}_{yyz} =
 -\sqrt{2\pi/105}Y_{3,2}
 -(2/5)\sqrt{\pi/7}Y_{3,0}
 -\sqrt{2\pi/105}Y_{3,-2}$\\
${\mathcal A}^{(3)}_{yyy} =
 -i\sqrt{\pi/35}Y_{3,3}
 -(i/5)\sqrt{3\pi/7}Y_{3,1}
 -(i/5)\sqrt{3\pi/7}Y_{3,-1}
 -i\sqrt{\pi/35}Y_{3,-3}$\\
${\mathcal A}^{(3)}_{xzz} =
 -(4/5)\sqrt{\pi/21}Y_{3,1}
 +(4/5)\sqrt{\pi/21}Y_{3,-1}$\\
${\mathcal A}^{(3)}_{xyz} =
 -i\sqrt{2\pi/105}Y_{3,2}
 +i\sqrt{2\pi/105}Y_{3,-2}$\\
${\mathcal A}^{(3)}_{xyy} =
\sqrt{\pi/35}Y_{3,3}
 +(1/5)\sqrt{\pi/21}Y_{3,1}
 -(1/5)\sqrt{\pi/21}Y_{3,-1}
 -\sqrt{\pi/35}Y_{3,-3}$\\
${\mathcal A}^{(3)}_{xxz} =
\sqrt{2\pi/105}Y_{3,2}
 -(2/5)\sqrt{\pi/7}Y_{3,0}
 +\sqrt{2\pi/105}Y_{3,-2}$\\
${\mathcal A}^{(3)}_{xxy} =
i\sqrt{\pi/35}Y_{3,3}
 -(i/5)\sqrt{\pi/21}Y_{3,1}
 -(i/5)\sqrt{\pi/21}Y_{3,-1}
 +i\sqrt{\pi/35}Y_{3,-3}$\\
${\mathcal A}^{(3)}_{xxx} =
 -\sqrt{\pi/35}Y_{3,3}
 +(1/5)\sqrt{3\pi/7}Y_{3,1}
 -(1/5)\sqrt{3\pi/7}Y_{3,-1}
 +\sqrt{\pi/35}Y_{3,-3}$\\
${\mathcal A}^{(4)}_{zzzz} =
(16/105)\sqrt{\pi}Y_{4,0}$\\
${\mathcal A}^{(4)}_{yzzz} =
(4i/21)\sqrt{\pi/5}Y_{4,1}
 +(4i/21)\sqrt{\pi/5}Y_{4,-1}$\\
${\mathcal A}^{(4)}_{yyzz} =
 -(2/21)\sqrt{2\pi/5}Y_{4,2}
 -(8/105)\sqrt{\pi}Y_{4,0}
 -(2/21)\sqrt{2\pi/5}Y_{4,-2}$\\
${\mathcal A}^{(4)}_{yyyz} =
 -(i/3)\sqrt{\pi/35}Y_{4,3}
 -(i/7)\sqrt{\pi/5}Y_{4,1}
 -(i/7)\sqrt{\pi/5}Y_{4,-1}
 -(i/3)\sqrt{\pi/35}Y_{4,-3}$\\
${\mathcal A}^{(4)}_{yyyy} =
(1/3)\sqrt{2\pi/35}Y_{4,4}
 +(2/21)\sqrt{2\pi/5}Y_{4,2}
 +(2/35)\sqrt{\pi}Y_{4,0}
 +(2/21)\sqrt{2\pi/5}Y_{4,-2}
 +(1/3)\sqrt{2\pi/35}Y_{4,-4}$\\
${\mathcal A}^{(4)}_{xzzz} =
 -(4/21)\sqrt{\pi/5}Y_{4,1}
 +(4/21)\sqrt{\pi/5}Y_{4,-1}$\\
${\mathcal A}^{(4)}_{xyzz} =
 -(2i/21)\sqrt{2\pi/5}Y_{4,2}
 +(2i/21)\sqrt{2\pi/5}Y_{4,-2}$\\
${\mathcal A}^{(4)}_{xyyz} =
(1/3)\sqrt{\pi/35}Y_{4,3}
 +(1/21)\sqrt{\pi/5}Y_{4,1}
 -(1/21)\sqrt{\pi/5}Y_{4,-1}
 -(1/3)\sqrt{\pi/35}Y_{4,-3}$\\
${\mathcal A}^{(4)}_{xyyy} =
(i/3)\sqrt{2\pi/35}Y_{4,4}
 +(i/21)\sqrt{2\pi/5}Y_{4,2}
 -(i/21)\sqrt{2\pi/5}Y_{4,-2}
 -(i/3)\sqrt{2\pi/35}Y_{4,-4}$\\
${\mathcal A}^{(4)}_{xxzz} =
(2/21)\sqrt{2\pi/5}Y_{4,2}
 -(8/105)\sqrt{\pi}Y_{4,0}
 +(2/21)\sqrt{2\pi/5}Y_{4,-2}$\\
${\mathcal A}^{(4)}_{xxyz} =
(i/3)\sqrt{\pi/35}Y_{4,3}
 -(i/21)\sqrt{\pi/5}Y_{4,1}
 -(i/21)\sqrt{\pi/5}Y_{4,-1}
 +(i/3)\sqrt{\pi/35}Y_{4,-3}$\\
${\mathcal A}^{(4)}_{xxyy} =
 -(1/3)\sqrt{2\pi/35}Y_{4,4}
 +(2/105)\sqrt{\pi}Y_{4,0}
 -(1/3)\sqrt{2\pi/35}Y_{4,-4}$\\
${\mathcal A}^{(4)}_{xxxz} =
 -(1/3)\sqrt{\pi/35}Y_{4,3}
 +(1/7)\sqrt{\pi/5}Y_{4,1}
 -(1/7)\sqrt{\pi/5}Y_{4,-1}
 +(1/3)\sqrt{\pi/35}Y_{4,-3}$\\
${\mathcal A}^{(4)}_{xxxy} =
 -(i/3)\sqrt{2\pi/35}Y_{4,4}
 +(i/21)\sqrt{2\pi/5}Y_{4,2}
 -(i/21)\sqrt{2\pi/5}Y_{4,-2}
 +(i/3)\sqrt{2\pi/35}Y_{4,-4}$\\
${\mathcal A}^{(4)}_{xxxx} =
(1/3)\sqrt{2\pi/35}Y_{4,4}
 -(2/21)\sqrt{2\pi/5}Y_{4,2}
 +(2/35)\sqrt{\pi}Y_{4,0}
 -(2/21)\sqrt{2\pi/5}Y_{4,-2}
 +(1/3)\sqrt{2\pi/35}Y_{4,-4}$\\
\end{document}
